prove progress modulo subT_of_algoSubT

TAPLFormalization/16-algo-subtyping/AST.lean
@@ -37,8 +37,6 @@ inductive WellFormed : Typ → Prop where
     (∀ ty ∈ tys, WellFormed ty) →
     WellFormed (.record labels tys)
 
--- abbrev WellFormedTyp := {T : Typ // WellFormed T}
-
 inductive Term where
   | var : ℕ → Term
   | app : Term → Term → Term
@@ -46,15 +44,26 @@ inductive Term where
   | record : SList → List Term → Term
   | proj : Term → String → Term
 
+def Term.recC {motive : Term → Sort u}
+  (var : ∀ {n}, motive (.var n))
+  (app : ∀ {t₁ t₂}, motive t₁ → motive t₂ → motive (.app t₁ t₂))
+  (abs : ∀ {t T}, motive t → motive (.abs T t))
+  (record : ∀ {ls ts}, (∀ t ∈ ts, motive t) → motive (.record ls ts))
+  (proj : ∀ {t s}, motive t → motive (.proj t s))
+  : ∀ t : Term, motive t
+  | .var n => var
+  | .app t₁ t₂ => app (t₁.recC var app abs record proj) (t₂.recC var app abs record proj)
+  | .abs T t => abs (t.recC var app abs record proj)
+  | .record ls ts => record (fun t _ => t.recC var app abs record proj)
+  | .proj t s => proj (t.recC var app abs record proj)
+
 @[grind]
 inductive IsVal : Term → Prop where
-  | is_abs : IsVal (Term.abs T t)
+  | abs : IsVal (Term.abs T t)
   | record :
-    ls.length == ts.length →
-    ∀ p ∈ ts, IsVal p →
+    ls.length = ts.length →
+    (∀ p ∈ ts, IsVal p) →
     IsVal (.record ls ts)
-
-abbrev Val : Type := { t : Term // IsVal t }
 
 abbrev TyCtx : Type := List Typ  -- maps var indices to their types
 
@@ -105,27 +114,24 @@ decreasing_by
 
 abbrev shiftDown := shiftDown' 0
 
-@[grind]
 inductive SmallStep : Term → Term → Prop where
   | app1 :
     SmallStep t₁ t₁' →
     SmallStep (.app t₁ t₂) (.app t₁' t₂)
-  | app2 : (IsVal v₁) →
+  | app2 : IsVal v₁ →
     SmallStep t₂ t₂' →
     SmallStep (.app v₁ t₂) (.app v₁ t₂')
   | appAbs : (IsVal v₂) →
     SmallStep (.app (.abs T₁₁ t₁₂) v₂) (shiftDown (sub (shift 0 1 v₂) t₁₂))
-  | projRcd {ls : SList} {l : Label} (i : ℕ) :
+  | projRcd (i : Fin ls.length) :
     IsVal (.record ls ts) →
-    ls[i]? = some l →
-    ts[i]? = some t →
+    (ls.length = ts.length) →
     SmallStep (.proj (.record ls ts) l) t
   | proj :
     SmallStep t₁ t₂ →
     SmallStep (.proj t₁ s) (.proj t₂ s)
-  | rcd (i : ℕ) :
-    (_ : ts[i]? = some t) →
-    ∀ _ : j < i, IsVal (ts[j]'(by grind)) →
+  | rcd (i : Fin ts.length) :
+    (∀ j (_ : j < i), IsVal (ts[j]'(by grind))) →
     SmallStep t t' →
     SmallStep (.record ls ts) (.record ls (ts.set i t'))
 
@@ -152,7 +158,7 @@ inductive SubT : Typ → Typ → Prop where
   | rcdDepth :
     (_ : ls.length = ts₁.length) →
     (_ : ls.length = ts₂.length) →
-    (∀ i, (_ : i < ls.length) → SubT (ts₁[i]'(by grind)) (ts₂[i]'(by grind))) →
+    (∀ i : Fin ls.length, SubT ts₁[i] ts₂[i]) →
     SubT (.record ls ts₁) (.record ls ts₂)
   | rcdPerm {ls ls' : SList} :
     (∀ ty ∈ tys, WellFormed ty) →
@@ -284,7 +290,19 @@ theorem algoSubT_of_subT : SubT S T → AlgoSubT S T := by
   case rcdDepth =>
     apply AlgoSubT.rcd
     case inj => exact id
-    all_goals grind [List.getElem?_of_mem]
+    any_goals grind [List.getElem?_of_mem, Fin]
+    · intro ty ty_mem
+      rename_i ts₁ ts₂ ls leneq₁ leneq₂ _ asubh
+      let ⟨i, ⟨h_i, ty_eq⟩⟩ := List.getElem_of_mem ty_mem
+      rw [← ty_eq]
+      rw [← leneq₁] at h_i
+      exact wf_of_algoSubT_left (asubh ⟨i, h_i⟩)
+    · intro ty ty_mem
+      rename_i ts₁ ts₂ ls leneq₁ leneq₂ _ asubh
+      let ⟨i, ⟨h_i, ty_eq⟩⟩ := List.getElem_of_mem ty_mem
+      rw [← ty_eq]
+      rw [← leneq₂] at h_i
+      exact wf_of_algoSubT_right (asubh ⟨i, h_i⟩)
   case rcdPerm tys tys' ls ls' tys_wf tys'_wf ls_eq tys_eq tys'_eq bij bij_h =>
     apply AlgoSubT.rcd
     case inj => exact fun i => bij ⟨i, by grind⟩
@@ -295,10 +313,19 @@ theorem algoSubT_of_subT : SubT S T → AlgoSubT S T := by
       rw [(bij_h ⟨i, by grind⟩).right]
       exact AlgoSubT.refl (by grind)
 
+lemma subT_of_rec_inj {ls ls' : SList} {tys tys' : List Typ} :
+  (_ : ls.length = tys.length) →
+  (_ : ls'.length = tys'.length) →
+  (inj : Fin ls.length → Fin ls'.length) →
+  (∀ i : Fin ls.length, ls[i] = ls'[inj i] ∧ tys[i] = tys'[inj i]) →
+  (.record ls' tys') <: (.record ls tys) := by
+  sorry
+
 theorem subT_of_algoSubT : AlgoSubT S T → SubT S T := by
   intro asub
   induction asub <;> try grind [SubT.top, SubT.arrow]
-  · sorry
+  case rcd ls₁ ls₂ tys₁ tys₂ tys₁_wf tys₂_wf leneq₁ leneq₂ inj inj_eq inj_asub inj_sub =>
+    sorry
 
 theorem algoSubT_iff_subT : AlgoSubT S T ↔ SubT S T :=
   .intro subT_of_algoSubT algoSubT_of_subT
@@ -330,4 +357,139 @@ theorem typing_of_algoTyping : AlgoTyping Γ t T → Typing Γ t T := by
   induction atyp <;> try grind [Typing, subT_of_algoSubT]
 
 theorem algoTyping_of_typing : Typing Γ t T → ∃ S, S <: T ∧ AlgoTyping Γ t S := by
-  sorry
+  intro typ
+  induction typ
+  case var T _ _ T_wf x_mem => exact ⟨T, ⟨.refl T_wf, .var T_wf x_mem⟩⟩
+  case abs T₁ Γ t₂ T₂ T₁_wf t₁_typ ih =>
+    let ⟨S₂, ⟨S₂_sub, t₂_typ⟩⟩ := ih
+    exists T₁.arrow S₂
+    constructor
+    · exact .arrow T₁_wf T₁_wf
+        (wf_of_algoSubT_right $ algoSubT_of_subT S₂_sub)
+        (wf_of_algoSubT_left $ algoSubT_of_subT S₂_sub)
+        (.refl T₁_wf) S₂_sub
+    · exact .abs T₁_wf t₂_typ
+  case app Γ t₁ T₁ T₂ t₂ t₁_typ t₂_typ ih₁ ih₂ =>
+    let ⟨S₁, ⟨sub₁, atyp₁⟩⟩ := ih₁
+    let ⟨S₂, ⟨sub₂, atyp₂⟩⟩ := ih₂
+    cases (algoSubT_of_subT sub₁)
+    rename_i Γ S₁ S₂' S₁_wf S₂'_wf T₁_wf asub₁ T₂_wf asub₂
+    exists S₂'
+    exact ⟨
+      subT_of_algoSubT asub₂,
+      .app atyp₁ atyp₂ (.trans (algoSubT_of_subT sub₂) asub₁)
+    ⟩
+  case sub Γ t S T' typ sub ih =>
+    let ⟨S', ⟨ssub, atyp⟩⟩ := ih
+    exact ⟨S', ⟨.trans ssub sub, atyp⟩⟩
+  case record Γ ts tys ls ts_len tys_len ts_typ ih =>
+    let tys' := (List.finRange ls.length).map (fun i => (ih i).choose)
+    exists .record ls tys'
+    exact ⟨
+      SubT.rcdDepth (ts₁ := tys') (ts₂ := tys) (ls := ls) (by grind) tys_len (by grind),
+      AlgoTyping.record ts_len (by grind) (by grind)
+    ⟩
+  case proj Γ r ls tys i leneq typ ih =>
+    let ⟨S, ⟨S_sub, atyp⟩⟩ := ih
+    cases (algoSubT_of_subT S_sub)
+    rename_i ls' tys' tys'_wf leneq' inj tys_wf _ inj_eq asub
+    rw [← inj_eq i]
+    exists tys'[inj i]
+    exact ⟨
+      subT_of_algoSubT $ asub i,
+      .proj (inj i) leneq' atyp
+    ⟩
+
+lemma canonical_form_arrow : AlgoTyping ∅ v (.arrow T₁ T₂) → IsVal v →
+  ∃ S t, v = .abs S t := by
+  intro atyp v_val
+  cases v_val <;> cases atyp
+  exact ⟨_, ⟨_, rfl⟩⟩
+
+lemma canonical_form_rcd : AlgoTyping ∅ v (.record ls tys) → IsVal v →
+  ∃ vs,
+  ls.length = vs.length ∧ (∀ p ∈ vs, IsVal p) ∧ v = .record ls vs := by
+  intro atyp v_val
+  cases v_val <;> cases atyp
+  rename_i ts ts_val ts_leneq _ tys_leneq ih
+  exists ts
+
+theorem algo_progress : (T : Typ) → AlgoTyping ∅ t T → IsVal t ∨ ∃ t', t ~> t' := by
+  apply Term.recC (motive := fun t => ∀ T, AlgoTyping ∅ t T → IsVal t ∨ ∃ t', t ~> t')
+  case var => intro n _ typ; cases typ; contradiction
+  case app =>
+    intro t₁ t₂ ih₁ ih₂ T t_atyp
+    apply Or.inr
+    cases t_atyp
+    rename_i T₁₁ T₂ asub t₂_atyp t₁_atyp
+    have ih₁' := ih₁ _ t₁_atyp
+    have ih₂' := ih₂ _ t₂_atyp
+    cases ih₁'
+    · cases ih₂'
+      · rename_i t₁_val t₂_val
+        let ⟨S, ⟨t₁₂, t₁_eq⟩⟩ := canonical_form_arrow t₁_atyp t₁_val
+        rw [t₁_eq]
+        exact ⟨_, SmallStep.appAbs t₂_val⟩
+      · rename_i t₁_val tst
+        let ⟨t₂', st⟩ := tst
+        exact ⟨_, SmallStep.app2 t₁_val st⟩
+    · rename_i tst
+      have ⟨t₁', st⟩ := tst
+      exact ⟨_, SmallStep.app1 st⟩
+  case abs =>
+    intro _ _ _ _ _
+    exact .inl .abs
+  case record =>
+    intro ls ts ih T atyp
+    cases atyp
+    rename_i tys tys_leneq ts_leneq ts_atyp
+    have ih' := fun (i : Fin ls.length) => ih ts[i] (by grind) _ (ts_atyp i)
+    induction ts generalizing ls tys with
+    | nil => exact .inl (.record ts_leneq (by grind))
+    | cons t ts' ts_ih =>
+      cases hls : ls.elems <;> try grind [SList.length]
+      rename_i l ls'_list
+      cases tys <;> try grind [SList.length]
+      rename_i ty tys'
+      rw [List.length] at ts_leneq tys_leneq
+      let ls' : SList := ⟨ls'_list, by grind [SList]⟩
+      have ls_leneq : ls.length = ls'.length + 1 := by grind [SList.length]
+      have ts_ih' := ts_ih (fun te _ T te_atyp => ih te (by grind) _ te_atyp)
+        (tys := tys') (ls := ls') (by grind [SList.length]) (by grind [SList.length])
+        (fun i => ts_atyp ⟨i + 1, by grind⟩)
+        (fun i => ih' ⟨i + 1, by grind⟩)
+      cases h : ih' ⟨0, by grind⟩
+      · rename_i t_val
+        cases ts_ih'
+        · exact .inl (.record (by grind) (by grind))
+        · rename_i tst
+          let ⟨t_', st⟩ := tst
+          cases st
+          apply Or.inr
+          rename_i r r' r_st i val_h
+          exact ⟨_, .rcd ⟨i + 1, by grind⟩ (fun j h_j => by
+            let ⟨j', _⟩ := j
+            cases j' <;> simp
+            case zero => assumption
+            case succ n _ => exact val_h ⟨n, by grind⟩ (by grind)
+          ) r_st⟩
+      · rename_i tst
+        let ⟨t', st⟩ := tst
+        exact .inr ⟨_, .rcd ⟨0, by grind⟩ (by grind) st⟩
+  · intro r s ih T atyp
+    cases atyp
+    rename_i ls tys i leneq r_atyp
+    let ih' := ih _ r_atyp
+    cases ih'
+    · rename_i r_val
+      let ⟨vs, ⟨vs_leneq, ⟨vs_val, r_eq⟩⟩⟩ := canonical_form_rcd r_atyp r_val
+      rw [r_eq]
+      exact .inr ⟨vs[i]'(by grind), .projRcd i (.record vs_leneq vs_val) vs_leneq⟩
+    · rename_i tst
+      let ⟨r', st⟩ := tst
+      exact .inr ⟨_, .proj st⟩
+
+theorem progress : (T : Typ) → Typing ∅ t T → IsVal t ∨ ∃ t', t ~> t' := by
+  intro T typ
+  let ⟨S, ⟨_, atyp⟩⟩ := algoTyping_of_typing typ
+  exact algo_progress S atyp
